library/init/data/sum/instances.lean
@@ -4,7 +4,7 @@ Released under Apache 2.0 license as described in the file LICENSE.
 Authors: Leonardo de Moura
 -/
 prelude
-import init.meta.mk_dec_eq_instance
+import init.meta.ttactic
 
 universes u v
 instance {α : Type u} {β : Type v} [decidable_eq α] [decidable_eq β] : decidable_eq (α ⊕ β) :=
